\documentclass[a4paper,12pt]{article}
\usepackage[english]{babel}
\usepackage[utf8x]{inputenc}
\usepackage[T1]{fontenc}
\usepackage[flushmargin]{footmisc}
\usepackage{setspace}
\usepackage[comma]{natbib}
\usepackage{float}
\usepackage{amsmath}
\usepackage{amsfonts}
\usepackage{amssymb}
\usepackage{ae}
\usepackage{caption}
\usepackage[a4paper,top=3cm,bottom=2cm,left=3cm,right=3cm,marginparwidth=1.75cm]{geometry}
\usepackage{graphicx}
\usepackage[colorinlistoftodos]{todonotes}
\usepackage[colorlinks=true, allcolors=blue]{hyperref}

\begin{document} \doublespacing \pagestyle{plain}
are identified:
\begin{equation} \begin{array}{rl} \displaystyle
 F_{Y_{1}(1,0)|\tau=c}(y) = \displaystyle \frac{p_{0|0}}{p_{0|0} - p_{0|1}}  F_{Q_{10}(Y_{0})|D=0,M=0}(y) \\ \displaystyle \qquad - \frac{p_{0|1}}{ p_{0|0} - p_{0|1}c}  F_{Y_1|D=1,M=0}(y), \end{array}
 \end{equation}
 \begin{equation}
 \begin{array}{rl}\displaystyle
F_{Y_{1}(0,0)|\tau=c}(y) = \displaystyle \frac{p_{0|0}}{p_{0|0} - p_{0|1}} F_{Y_{1}|D=0,M=0}(y) \\ \displaystyle \qquad - \frac{p_{0|1} }{p_{0|0} - p_{0|1}}F_{Q_{00}(Y_{0})|D=1,M=0}(y)  . 
\end{array}
\end{equation}
Therefore, the direct quantile effect under $d = 0$ on compliers, $\theta_1^{c}(q,0) = F_{Y_{1}(1,0)|c}^{-1}(q)-F_{Y_{1}(0,0)|c}^{-1}(q)$, is identified.
\textbf{Proof.} See Appendix .
\noindent \textbf{Theorem 4:} Under Assumptions 1â€“2, 5, 7-8,
\begin{itemize}
\item[a)] and Assumption 6a, the average and quantile direct effects on
always-takers are identified:
\begin{equation*}
\theta_1^a= \theta_1^{0,1}(0) \mbox{ and } \theta_1^a(q)= \theta_1^{0,1}(q,0).
\end{equation*}
\item[b)] and Assumption 6, the average direct effect under $d = 1$ on compliers is identified:
\begin{align*}
\theta_{1}^{c}(1) = \frac{p_{1|1}}{ p_{1|1} - p_{1|0}} \theta_1^{1,1}(1) -\frac{p_{1|0}}{p_{1|1} - p_{1|0}}\theta_1^{0,1}(0).
\end{align*}
Furthermore, the potential outcome distributions under $d = 1$ for compliers are identified:
\begin{equation} \begin{array}{rl} \displaystyle
 F_{Y_{1}(1,1)|\tau=c}(y) = \displaystyle \frac{p_{1|1}}{p_{1|1} - p_{1|0}} F_{Y_{1}|D=1,M=1}(y) \\ \displaystyle \qquad - \frac{p_{1|0} }{p_{1|1} - p_{1|0}}F_{Q_{11}(Y_0)|D=0,M=1}(y),  \end{array}
 \end{equation}
 \begin{equation}
 \begin{array}{rl}\displaystyle
F_{Y_{1}(0,1)|\tau=c}(y) =\displaystyle \frac{p_{1|1}}{p_{1|1} - p_{1|0}}  F_{Q_{01}(Y_{0})|D=1,M=1}(y)\\  \displaystyle \qquad - \frac{p_{1|0}}{ p_{1|1} - p_{1|0}}  F_{Y_1|D=0,M=1}(y).  \end{array}
\end{equation}
Therefore, the direct quantile effect under $d = 1$ on compliers $\theta_1^{c}(q,1) = F_{Y_{1}(1,1)|c}^{-1}(q)-F_{Y_{1}(0,1)|c}^{-1}(q)$ is identified.
\end{itemize}
\end{document}
