\documentclass[a4paper,12pt]{article}
\usepackage[english]{babel}
\usepackage[utf8x]{inputenc}
\usepackage[T1]{fontenc}
\usepackage[flushmargin]{footmisc}
\usepackage{setspace}
\usepackage[comma]{natbib}
\usepackage{float}
\usepackage{amsmath}
\usepackage{amsfonts}
\usepackage{amssymb}
\usepackage{ae}
\usepackage{caption}
\usepackage[a4paper,top=3cm,bottom=2cm,left=3cm,right=3cm,marginparwidth=1.75cm]{geometry}
\usepackage{graphicx}
\usepackage[colorinlistoftodos]{todonotes}
\usepackage[colorlinks=true, allcolors=blue]{hyperref}

\begin{document} \doublespacing \pagestyle{plain}
Under Assumption 7 and 8,
\begin{equation}  \begin{array}{rl} E[1\{Y_1(0,0) \leq y\}|D=1,M(1)=0]\stackrel{A7,A8}{=}E[1\{Y_1(0,0) \leq y\}|\tau=n]\\  = F_{Y_{1}(0,0)|\tau=n}(y),
\end{array} \end{equation}
which proves.
\subsection{Average direct effect under $\mathbf{d = 0}$ on compliers}
In the following, we show that
\begin{align*}
\displaystyle \theta_1^{c}(0) = E[Y_1(1,0)-Y_1(0,0)|\tau=c], \\ =
\frac{p_{0|0}}{p_{0|0} - p_{0|1}}E[Q_{10}(Y_0)- Y_1|D=0,M=0] \\
  - \frac{p_{0|1}}{p_{0|0} - p_{0|1}}E[Y_1 - Q_{00}(Y_0)|D=1,M=0].
\end{align*}
Plugging () in () under $T=1$, we obtain
\begin{equation*}
\begin{array}{rl}
E[Y_1|D=0,M=0]  = \displaystyle  \frac{p_n}{p_n + p_c}E[Q_{00}(Y_0)|D=1,M=0] \\
\displaystyle \quad +   \frac{p_c}{p_n + p_c}E[Y_1(0,0)|\tau=c].
\end{array}
\end{equation*}
This allows identifying
\begin{equation} 
\begin{array}{rl}
E[Y_1(0,0)|\tau=c] = \displaystyle \frac{p_{0|0}}{ p_{0|0} - p_{0|1}} E[Y_1|D=0,M=0] \\
 \displaystyle \quad -\frac{p_{0|1}}{p_{0|0} - p_{0|1}}E[Q_{00}(Y_0)|D=1,M=0].
\end{array}
\end{equation}
Accordingly, we have to show the identification of $E[Y_1(1,0)|c]$ to finish the proof. From () we have $E[Y_1(1,0)|D=0,M=0] = E[Q_{10}(Y_0)|D=0,M=0]$. Applying
\end{document}
