\documentclass[a4paper,12pt]{article}
\usepackage[english]{babel}
\usepackage[utf8x]{inputenc}
\usepackage[T1]{fontenc}
\usepackage[flushmargin]{footmisc}
\usepackage{setspace}
\usepackage[comma]{natbib}
\usepackage{float}
\usepackage{amsmath}
\usepackage{amsfonts}
\usepackage{amssymb}
\usepackage{ae}
\usepackage{caption}
\usepackage[a4paper,top=3cm,bottom=2cm,left=3cm,right=3cm,marginparwidth=1.75cm]{geometry}
\usepackage{graphicx}
\usepackage[colorinlistoftodos]{todonotes}
\usepackage[colorlinks=true, allcolors=blue]{hyperref}

\begin{document} \doublespacing \pagestyle{plain}
 \subsection{Quantile direct effect on the
always-takers}
We prove that
\begin{align*}
\theta_1^a (q) = F_{Y_1(1,1)|\tau=a}^{-1}(q)- F_{Y_1(0,1)|\tau=a}^{-1}(q), \\
= F_{Q_{11}(Y_0)|D=0,M=1}^{-1}(q)-F_{Y_1|D=0,M=1}^{-1}(q).
\end{align*}
This requires showing that
\begin{align}
F_{Y_1(1,1)|\tau=a}(y) =F_{Q_{11}(Y_0)|D=0,M=1}(y) \mbox{ and} \\
F_{Y_1(0,1)|\tau=a}(y)  = F_{Y_1|D=0,M=1}(y). 
\end{align}
Under Assumptions 7 and 8,
\begin{equation} 
\begin{array}{rl}
F_{Y_t|D=0,M=1} (y) = E[1\{Y_t\leq y\}|D=0,M=1] \\ \stackrel{A7,A8}{=}E[1\{Y_t(0,1)\leq y\}|\tau=a] \\ = F_{Y_{t}(0,1)|\tau=a}, (y). \end{array}
\end{equation}
which proves (). From (), we have
\begin{equation*}
F_{Q_{11}(Y_{0})|D=0,M=1}(y) = F_{Y_{1}(1,1)|D=0,M(0)=1}(y)=E[1\{Y_1(1,1) \leq y\}|D=0,M(0)=1].
\end{equation*}
Under Assumption 7 and 8,
\begin{equation}  \begin{array}{rl} E[1\{Y_1(1,1) \leq y\}|D=0,M(0)=1]\stackrel{A7,A8}{=}E[1\{Y_1(1,1) \leq y\}|\tau=a]\\  = F_{Y_1(1,1)|\tau=a}(y),
\end{array} \end{equation}
which proves.
\end{document}
