\documentclass[a4paper,12pt]{article}
\usepackage[english]{babel}
\usepackage[utf8x]{inputenc}
\usepackage[T1]{fontenc}
\usepackage[flushmargin]{footmisc}
\usepackage{setspace}
\usepackage[comma]{natbib}
\usepackage{float}
\usepackage{amsmath}
\usepackage{amsfonts}
\usepackage{amssymb}
\usepackage{ae}
\usepackage{caption}
\usepackage[a4paper,top=3cm,bottom=2cm,left=3cm,right=3cm,marginparwidth=1.75cm]{geometry}
\usepackage{graphicx}
\usepackage[colorinlistoftodos]{todonotes}
\usepackage[colorlinks=true, allcolors=blue]{hyperref}

\begin{document} \doublespacing \pagestyle{plain}
\subsection{Average direct effect
under $\mathbf{d = 1}$ on compliers}
In the following, we show that
\begin{align*}
\theta_{1}^{c}(1) = E[Y_1(1,1)-Y_1(0,1)|\tau=c], \\ = 
\frac{p_{1|1}}{ p_{1|1} - p_{1|0}} E[Y_1-Q_{01}(Y_0) |D=1,M=1] \\ -\frac{p_{1|0}}{p_{1|1} - p_{1|0}}E[Q_{11}(Y_0)-Y_1|D=0,M=1].
\end{align*}
Plugging () in (), we obtain
\begin{equation*}
\begin{array}{rl}
E[Y_1|D=1,M=1] = \displaystyle \frac{p_a}{p_a + p_c}E[Q_{11}(Y_0)|D=0,M=1] \\
 \displaystyle \quad + \frac{p_c}{p_a + p_c} E[Y_1(1,1)|\tau=c].
\end{array}
\end{equation*}
This allows identifying
\begin{equation} 
\begin{array}{rl}
E[Y_1(1,1)|\tau=c] = \displaystyle \frac{p_{1|1}}{ p_{1|1} - p_{1|0}} E[Y_1|D=1,M=1] \\
 \displaystyle \quad -\frac{p_{1|0}}{p_{1|1} - p_{1|0}}E[Q_{11}(Y_0)|D=0,M=1].
\end{array}
\end{equation}
From () we have $E[Y_1(0,1)|D=1,M=1] = E[Q_{01}(Y_0)|D=1,M=1]$. Applying the law of iterative expectations, gives
\begin{align*}
E[Y_1(0,1)|D=1,M=1] = \frac{p_a}{p_a+p_c} E[Y_1(0,1)|D=1,M=1, \tau=a] \\+ \frac{p_c}{p_a+p_c}E[Y_1(0,1)|D=1,M=1,\tau= c], \\
\stackrel{A7}{=} \frac{p_a}{p_a+ p_c} E[Y_1(0,1)|\tau=a] + \frac{p_c}{p_a+p_c}E[Y_1(0,1)|\tau= c].
\end{align*}
After some rearrangements and using (), we obtain
\begin{equation*}
E[Y_1(0,1)|\tau= c]  = \frac{p_a+p_c}{p_c} E[Q_{01}(Y_0)|D=1,M=1] -   \frac{p_a}{p_c} E[Y_1|D=0,M=1].
\end{equation*}
\end{document}
